\\\Large\text{188}\normalsize\\
x^3-5x^2+14x-16=0, x\in\Z\\
x\in\{t:t\mid -16\}\\
x\in\{\pm16,\pm8,\pm4,\pm2,\pm1\}\\
x=2
\\\Large\text{189}\normalsize\\
x^4-2x^3+2x^2-22x+21=0,x\in\Z\\
x\in\{t:t\mid 21\}\\
x\in\{\pm21,\pm7,\pm3,\pm1\}\\
x_1=1,x_2=3
\\\Large\text{190}\normalsize\\
x^5+5x^4+6x^3-x^2-5x-6=0,x\in\Z\\
x\in\{t:t\mid -6\}\\
x\in\{\pm6,\pm3,\pm2,\pm1\}\\
x_1=-3,x_2=-2,x_3=1
\\\Large\text{191}\normalsize\\
P=x^3-6x^2+11x-6=(x-1)(x-2)(x-3)\\
Q=x^3+3x^2-25x+21=(x-1)(x-3)(x+7)\\
\gcd(P,Q)=(x-1)(x-3)=x^2-4x+3
\\\Large\text{192}\normalsize\\
P=x^3-9x^2+23x-15=(x-1)(x-3)(x-5)\\
Q=x^3-5x^2-28x+32=(x-1)(x+4)(x-8)\\
\gcd(P,Q)=x-1
\\\Large\text{193}\normalsize\\
\frac{a(x)}{b(x)}=\frac{8x^3-x^2-10x+2}{x+1}\\
q(x)=8x^2-9x-1
\\\Large\text{194}\normalsize\\
\frac{10(-2x-9)}{x^2+12x+11}=
\frac{-10(2x+9)}{(x+11)(x+1)}=
\frac{A}{x+11}+\frac{B}{x+1}\\
-20x-90=(A+B)x+A+11B\\
A=-13; B=-7\\
\frac{-13}{x+11}+\frac{-7}{x+1}
\\\Large\text{195}\normalsize\\
\frac{2x^2+13x+37}{(x+6)(x^2+12x+36)}=
\frac{2x^2+13x+37}{(x+6)^3}=
\frac{A_3}{(x+6)^3}+\frac{A_2}{(x+6)^2}+\frac{A_1}{x+6}\\
2x^2+13x+37=A_3+A_2(x+6)+A_1(x^2+12x+36)=\\
A_1 x^2+(A_2+12 A_1)x+(A_3+6 A_2 + 36 A_1)\\
A_1=2;A_2=-11;A_3=31\\
\frac{31}{(x+6)^3}+\frac{-11}{(x+6)^2}+\frac{2}{x+6}
\\\Large\text{196}\normalsize\\
\frac{2x^2+12x-18}{(x+6)^2(x+8)}=
\frac{A_2}{(x+6)^2}+\frac{A_1}{x+6}+\frac{B}{x+8}\\
2x^2+12x-18=A_2(x+8)+A_1(x^2+14x+48)+B(x^2+12x+36)=\\
(A_1+B)x^2+(A_2+14A_1+12B)x+(8A_2+48A_1+36B)\\
A_1=\frac{-3}{2};B=\frac{7}{2};A_2=-9\\
\frac{-9}{(x+6)^2}+\frac{-3}{2(x+6)}+\frac{7}{2(x+8)}
\\\Large\text{197}\normalsize\\
\frac{9(x^2+6x+5)}{(x+4)(x^2+8x+25)}=
\frac{A}{x+4}+\frac{Px+Q}{x^2+8x+25}\\
9x^2+54x+45=Ax^2+8Ax+25A+Px^2+(4P+Q)x+4Q=\\
(A+P)x^2+(8A+4P+Q)x+(25A+4Q)\\
A=-3;Q=30;P=12\\
\frac{6(2x+5)}{x^2+8x+25}+\frac{-3}{x+4}
\\\Large\text{198}\normalsize\\
\frac{(x^2+8x+2)}{(x+4)(x+3)(x+2)}=
\frac{A}{x+4}+\frac{B}{x+3}+\frac{C}{x+2}\\
x^2+8x+2=A(x^2+5x+6)+B(x^2+6x+8)+C(x^2+7x+12)=\\
(A+B+C)x^2+(5A+6B+7C)x+(6A+8B+12C)\\
A=-7;B=13;C=-5\\
\frac{-7}{x+4}+\frac{13}{x+3}+\frac{-5}{x+2}
\\\Large\text{199}\normalsize\\
\frac{x^6+4x^5-11x^4-44x^3-8x^2+16x-18}{x^4+2x^3-13x^2-14x+24}=\\
x^2+2x-2+\frac{-30(x^2+2x-1)}{(x-1)(x+2)(x-3)(x+4)}=\\
x^2+2x-2+\frac{A}{x-1}+\frac{B}{x+2}+\frac{C}{x-3}+\frac{D}{x+4}\\
-30(x^2+2x-1)=A(x^3+3x^2-10x-24)+\\
B(x^3-13x+12)+C(x^3+5x^2+2x-8)+\\
D(x^3-2x^2-5x+6)=\\
(A+B+C+D)x^3+(3A+5C-2D)x^2+\\
(-10A-13B+2C-5D)x+(-24A+12B-8C+6D)\\
\begin{cases}
A+B+C+D=0&(1)\\
3A+0B+5C-2D=-30&(2)\\
-10A-13B+2C-5D=-60&(3)\\
-24A+12B-8C+6D=30&(4)
\end{cases}\\
(1)+(2)+(3)+(4):\\
-30A=-60\rArr A=2\\
\begin{cases}
B+C+D=-2&(1)\\
5C-2D=-36&(2)\\
-13B+2C-5D=-40&(3)\\
6B-4C+3D=39&(4)
\end{cases}\\
(2)+(4)-(1):\\
5B=5\rArr B=1\\
\begin{cases}
C+D=-3&(1)\\
5C-2D=-36&(2)
\end{cases}\\
(2)+2\cdot(1):\\
7C=-42\rArr C=-6; D=3\\
x^2+2x-2+\frac{2}{x-1}+\frac{1}{x+2}+\frac{-6}{x-3}+\frac{3}{x+4}
\\\Large\text{200}\normalsize\\
\frac{-x^6+2x^4+5x^3-2x^2+11x-2}{x^4+x^3-2x^2-16x+16}=\\
-x^2+x-1+\frac{-8x^3+28x^2-21x+14}{(x-1)(x-2)(x^2+4x+8)}=\\
-x^2+x-1+\frac{A}{x-1}+\frac{B}{x-2}+\frac{Px+Q}{x^2+4x+8}\\
-8x^3+28x^2-21x+14=\\
A(x^3+2x^2-16)+B(x^3+3x^2+4x-8)+(Px+Q)(x^2-3x+2)=\\
(A+B+P)x^3+(2A+3B-3P+Q)x^2+\\
(4B+2P-3Q)x+(-16A-8B+2Q)\\
\begin{cases}
A+B+P=-8&(1)\\
2A+3B-3P+Q=28&(2)\\
4B+2P-3Q=-21&(3)\\
-16A-8B+2Q=14&(4)
\end{cases}\\
(1)+(2)+(3)+(4):\\
-13A=13\rArr A=-1\\
\begin{cases}
B+P=-7&(1)\\
3B-3P+Q=30&(2)\\
4B+2P-3Q=-21&(3)\\
-8B+2Q=-2&(4)
\end{cases}\\
2\cdot(2)+6\cdot(1)-(4):\\
20B=20\rArr B=1;P=-8;Q=3\\
-x^2+x-1+\frac{-1}{x-1}+\frac{1}{x-2}+\frac{-8x+3}{x^2+4x+8}
\\\Large\text{201}\normalsize\\
\frac{3i+4}{5i-3}=\frac{(3i+4)(5i+3)}{-25-9}=\frac{-15+20i+9i+12}{-34}=\\
\frac{3}{34}-\frac{29}{34}i
\\\Large\text{202}\normalsize\\
\frac{(-3+5i)(6+i)}{2+i}=\frac{(-23+27i)(2-i)}{3}=\\
\frac{-19}{3}+\frac{77}{3}i
\\\Large\text{203}\normalsize\\
P(z)=(-1+5i)z^2+(6-6i)z+(5-2i);z=-4+6i\\
P(z)=(-1+5i)(-4+6i)^2+(6-6i)(-4+6i)+(5-2i)=\\
(-1+5i)(-20-48i)+(12+60i)+(5-2i)=\\
(260-52i)+(12+60i)+(5-2i)=\\
277+6i
\\\Large\text{204}\normalsize\\
z_1=-1-i; z_2=3-4i\\
\frac{z_1}{\overline{z_2}}-\frac{\overline{z_2}}{z_1}=
\frac{-1-i}{3+4i}-\frac{3+4i}{-1-i}=\\
\frac{(-1-i)(3-4i)}{9+16}-\frac{(3+4i)(-1+i)}{1+1}=\\
\frac{-7+i}{25}-\frac{-7-i}{2}=\\
\frac{161}{50}+\frac{27}{50}i
\\\Large\text{205}\normalsize\\
z_1=1-3i;z_2=2-i\\
\frac{\overline{z_1}+z_2}{z_1-\overline{z_2}}=
\frac{1+3i+2-i}{1-3i-2-i}=
\frac{3+2i}{-1-4i}=\\
\frac{(3+2i)(-1+4i)}{1+16}=\\
\frac{-11}{17}+\frac{10}{17}i
\\\Large\text{206}\normalsize\\
z=-2-2\sqrt{3}i\\
|z|=\sqrt{{-2}^2+(-2\sqrt{3})^2}=\sqrt{4+12}=4\\
\arg{z}=\arctan{\frac{-2\sqrt{3}}{-2}}=\frac{\pi}{3}
\\\Large\text{207}\normalsize\\
u=2(\cos{\frac{\pi}{4}}+i\sin{\frac{\pi}{4}});
v=3(\cos{\frac{\pi}{2}}+i\sin{\frac{\pi}{2}})\\
z=\frac{u^5}{\overline{v}^6}=
\frac{2^5(\cos{\frac{5\pi}{4}}+i\sin{\frac{5\pi}{4}})}
{3^6(\cos{-3\pi}+i\sin{-3\pi})}=\\
\frac{32(-\frac{1}{\sqrt{2}}-\frac{1}{\sqrt{2}}i)}{729(-1+0i)}=\\
\frac{16\sqrt{2}}{729}(1+i)\\
|z|=\frac{32}{729}\\
\arg{z}=\arctan{1}=\frac{\pi}{4}
\\\Large\text{208}\normalsize\\
u=3(\cos{\frac{\pi}{6}}+i\sin{\frac{\pi}{6}});
v=4(\cos{\frac{\pi}{7}}+i\sin{\frac{\pi}{7}})\\
z=\overline{u}^4\cdot\overline{v}^5=
81(\cos{\frac{-2\pi}{3}}+i\sin{\frac{-2\pi}{3}})\cdot
1024(\cos{\frac{-5\pi}{7}}+i\sin{\frac{-5\pi}{7}})=\\
82944(\cos{\frac{-29\pi}{21}}+i\sin{\frac{-29\pi}{21}})\\
|z|=82944;\arg z=\frac{13\pi}{21}
\\\Large\text{209}\normalsize\\
z=-1+\sqrt{3}i\\
|z|=\sqrt{1+3}=2;
\arg{z}=\arctan{-\sqrt{3}}=\frac{-\pi}{3}\\
z=2(\cos{\frac{-\pi}{3}}+i\sin{\frac{-\pi}{3}})
\\\Large\text{210}\normalsize\\
z=4(\cos{\pi}+i\sin{\pi})=-4
\\\Large\text{211}\normalsize\\
z^6=64; z\in\cnums\\
r^6(\cos{6\varphi}+i\sin{6\varphi})=64\\
\varphi=\pm\frac{2\pi}{6}\\
-r^6=64\rArr r=\pm2\\
z=\pm2(\frac{1}{2}\pm i\frac{\sqrt{3}}{2})\\
z\in\{2,-2,1+\sqrt{3}i,-1+\sqrt{3}i,1-\sqrt{3}i,-1-\sqrt{3}i\}
\\\Large\text{212}\normalsize\\
x^2+4x+20=0\\
x=\frac{-4\pm\sqrt{16-4\cdot20}}{2}=-2\pm4i
\\\Large\text{213}\normalsize\\
(1+4i)z^2+(18-13i)z-21-33i=0\\
x=\frac{-18+13i\pm\sqrt{(18-13i)^2+4(1+4i)(21+33i)}}{2+8i}=\\
x=\frac{-18+13i\pm\sqrt{155-468i-444+468i}}{2+8i}=\\
x=\frac{-18+13i\pm17i}{2+8i}=\\
\frac{(-18+13i\pm17i)(2-8i)}{68}\\
x_1=\frac{204+204i}{68}=3+3i\\
x_2=\frac{-68+136i}{68}=-1+2i
\\\Large\text{214}\normalsize\\
f(a,b,c)=a(-1-i)^2+b(-1-i)+c=0; a,b,c\in\R\\
2ai-b-bi+c=0\\
c-b+(2a-b)i=0\\
c-b=2a-b=0\\
c=b=2a\\
\#f^{-1}(\{0\})=\aleph_0\\
\{1,2,2\}\in f^{-1}(\{0\})\text{ :}\\
1(-1-i)^2+2(-1-i)+2=0
\\\Large\text{215}\normalsize\\
z^4+8z^3-2z^2-124z-240=0;z_1=-3-i\\
(-3-i)^2+b(-3-i)+c=0\\
8+6i-3b-bi+c=0\\
b=6;c=10\\
\frac{z^4+8z^3-2z^2-124z-240}{z^2+6z+10}=z^2+2z-24\\
(z+3+i)(z+3-i)(z+6)(z-4)=0\\
z_2=-3+i;z_3=-6;z_4=4
\\\Large\text{1004}\normalsize\\
\lim_{n\to\infty}{\bigg(\frac{2-7n+8n^2}{8n-8}+
\frac{5-2n-8n^2}{8n+6}\bigg)}=\\
\lim_{n\to\infty}{\frac{64n^3-8n^2-26n+12-64n^3+48n^2+56n-40}{64n^2-64}}=\\
\lim_{n\to\infty}{\frac{40n^2+30n-28}{64n^2-64}}=\frac{40}{64}=\frac{5}{8}\\
\\\Large\text{1031}\normalsize\\
\lim_{x\to\infty}{\frac{2x^2+5x-3}{9x^2-8}}=\frac{2}{9}\\
\\\Large\text{1032}\normalsize\\
\lim_{x\to\infty}{\frac{9x-3}{5\sin{4x}+9x+5}}=1\\
|\sin|\le1
\\\Large\text{1033}\normalsize\\
\lim_{x\to-\infty}{\frac{7\cdot7^x-3}{7\cdot7^x-5}}=\frac{3}{5}
\\\Large\text{1034}\normalsize\\
\lim_{x\to-\infty}{\frac{7\cdot8^x+5\cdot5^x}{2\cdot5^x-2\cdot8^x}}=\\
\lim_{x\to-\infty}{\frac{7\cdot(\frac{8}{5})^x+5}{2-2\cdot(\frac{8}{5})^x}}=
\frac{5}{2}
\\\Large\text{1035}\normalsize\\
\lim_{x\to+\infty}{\frac{8-5\cdot6^x}{3\cdot6^x-4}}=\\
\lim_{x\to+\infty}{\frac{8\cdot6^{-x}-5}{3-4\cdot6^{-x}}}=-\frac{5}{3}
\\\Large\text{1036}\normalsize\\
\lim_{x\to+\infty}{\frac{5\cdot4^x-5\cdot7^x}{6\cdot7^x-8\cdot4^x}}=\\
\lim_{x\to+\infty}{\frac{5\cdot(\frac{4}{7})^x-5}{6-8\cdot(\frac{4}{7})^x}}=
-\frac{5}{6}
\\\Large\text{1037}\normalsize\\
\lim_{x\to-\infty}{\Big(\sqrt{x(x+3)}-\sqrt{x^2-6}\Big)}=\\
\lim_{x\to-\infty}{\Bigg(
\frac{\cancel{x^2+}3x\cancel{-x^2}+6}
{\sqrt{x(x+3)}+\sqrt{x^2-6}}
\Bigg)}=\\
\lim_{x\to-\infty}{\Bigg(
\frac{3\cancel{+\frac{6}{x}}}
{-\sqrt{1\cancel{+\frac{3}{x}}}-\sqrt{1\cancel{-\frac{6}{x^2}}}}
\Bigg)}=-\frac{3}{2}
\\\Large\text{1038}\normalsize\\
\lim_{x\to+\infty}{\sqrt{x}\Big(\sqrt{8x+7}-\sqrt{8x-7}\Big)}=\\
\lim_{x\to+\infty}{\sqrt{x}\Bigg(
\frac{\cancel{8x+}7\cancel{-8x}+7}{\sqrt{8x+7}+\sqrt{8x-7}}
\Bigg)}=\\
\lim_{x\to+\infty}{\Bigg(
\frac{14\sqrt{x}}{\sqrt{8x+7}+\sqrt{8x-7}}
\Bigg)}=\\
\lim_{x\to+\infty}{\Bigg(
\frac{14}{\sqrt{8\cancel{+\frac{7}{x}}}+\sqrt{8\cancel{-\frac{7}{x}}}}
\Bigg)}=\frac{14}{4\sqrt{2}}=\frac{7\sqrt{2}}{4}
\\\Large\text{1039}\normalsize\\
\lim_{x\to-\infty}{(\sqrt{9x^2+x-4}-\sqrt{9x^2+2x-1})}=\\
\lim_{x\to-\infty}{\Bigg(
\frac{9x^2+x-4-9x^2-2x+1}
{\sqrt{9x^2+x-4}+\sqrt{9x^2+2x-1}}
\Bigg)}=\\
\lim_{x\to-\infty}{\Bigg(
\frac{-x-3}
{\sqrt{9x^2+x-4}+\sqrt{9x^2+2x-1}}
\Bigg)}=\\
\lim_{x\to-\infty}{\Bigg(
\frac{1+\frac{3}{x}}
{\sqrt{9+\frac{1}{x}-\frac{4}{x^2}}+\sqrt{9+\frac{2}{x}-\frac{1}{x^2}}}
\Bigg)}=\frac{1}{6}
\\\Large\text{1040}\normalsize\\
\lim_{x\to+\infty}{(\sqrt{2x^2-2x-4}-\sqrt{2x^2-3x+3})}=\\
\lim_{x\to+\infty}{\Bigg(
\frac{2x^2-2x-4-2x^2+3x-3}
{\sqrt{2x^2-2x-4}+\sqrt{2x^2-3x+3}}
\Bigg)}=\\
\lim_{x\to+\infty}{\Bigg(
\frac{x-7}
{\sqrt{2x^2-2x-4}+\sqrt{2x^2-3x+3}}
\Bigg)}=\\
\lim_{x\to+\infty}{\Bigg(
\frac{1-\frac{7}{x}}
{\sqrt{2-\frac{2}{x}-\frac{4}{x^2}}+\sqrt{2-\frac{3}{x}+\frac{3}{x^2}}}
\Bigg)}=\frac{1}{2\sqrt{2}}=\frac{\sqrt{2}}{4}
\\\Large\text{1041}\normalsize\\
\lim_{x\to+\infty}{\Big((\sqrt{2x^2-2}-\sqrt{2x^2+2})\arctan(5x-2)\Big)}=\\
\frac{\pi}{2}\lim_{x\to+\infty}{(\sqrt{2x^2-2}-\sqrt{2x^2+2})}=\\
\frac{\pi}{2}\lim_{x\to+\infty}{\Bigg(
\frac{\cancel{2x^2}-2\cancel{-2x^2}-2}
{\sqrt{2x^2-2}+\sqrt{2x^2+2}}
\Bigg)}=\frac{c}{\infty}=0
\\\Large\text{1042}\normalsize\\
\lim_{x\to+\infty}{\frac{-x^2+3x+1}{e^{-x}}}=\\
\lim_{x\to+\infty}{e^x}\lim_{x\to+\infty}{(-x^2+3x+1)}=\\
\infty\lim_{x\to+\infty}{-x^2}=\infty(-\infty)=-\infty
\\\Large\text{1046}\normalsize\\
\lim_{x\to1}{\frac{4x^2-x-3}{2x^2+2x-4}}=\\
\lim_{x\to1}{\frac{(4x+3)(x-1)}{2(x+2)(x-1)}}=\\
\lim_{x\to1}{\frac{4\cdot1+3}{2(1+2)}}=\frac{7}{6}
\\\Large\text{1047}\normalsize\\
\lim_{x\to-2}{\frac{4x^2-3x-22}{x^3+8}}=\\
\lim_{x\to-2}{\frac{(x+2)(4x-11)}{(x+2)(x^2-2x+4)}}=\\
\lim_{x\to-2}{\frac{4(-2)-11}{(-2)^2-2(-2)+4}}=-\frac{19}{12}
\\\Large\text{1048}\normalsize\\
\lim_{x\to8}{\frac{5x-40}{5-\sqrt{8x-39}}}=\\
\lim_{x\to8}{\frac{(5x-40)(5+\sqrt{8x-39})}{25-8x+39}}=\\
\lim_{x\to8}{\frac{5(x-8)(5+\sqrt{8x-39})}{8(8-x)}}=\\
\lim_{x\to8}{\frac{-5}{8}}(5+\sqrt{8x-39})=
\frac{-5}{8}(5+5)=-\frac{25}{4}
\\\Large\text{1049}\normalsize\\
\lim_{x\to2}{\frac{2x+1-\sqrt{2x^2+2x+13}}{\sqrt{4x^2+4x-8}+4x-12}}=\\
\lim_{x\to2}{\frac{2x+1-\sqrt{2x^2+2x+13}}{2\sqrt{(x+2)(x-1)}+(4x-12)}}=\\
\lim_{x\to2}
{\frac{(2x+1-\sqrt{2x^2+2x+13})(2\sqrt{(x+2)(x-1)}-4x+12)}
{4(x+2)(x-1)-(16x^2-96x+144)}}=\\
\lim_{x\to2}
{\frac{2(2x+1-\sqrt{2x^2+2x+13})(\sqrt{(x+2)(x-1)}-2x+6)}
{-12x^2+100x-152}}=\\
\lim_{x\to2}
{\frac{2(2x+1-\sqrt{2x^2+2x+13})(\sqrt{(x+2)(x-1)}-2x+6)}
{-4(x-2)(3x-19)}}=\\
\lim_{x\to2}
{\frac{2(2x+1-\sqrt{2x^2+2x+13})(\sqrt{(2+2)(2-1)}-2\cdot2+6)}
{-4(x-2)(3\cdot2-19)}}=\\
-\frac{2}{13}\lim_{x\to2}
{\frac{2x+1-\sqrt{2x^2+2x+13}}
{x-2}}=\\
-\frac{2}{13}\lim_{x\to2}
{\frac{2-\frac{2x+1}{\sqrt{2x^2+2x+13}}}
{1}}=\\
-\frac{2}{13}\lim_{x\to2}
{\frac{2-\frac{4+1}{5}}
{1}}=-\frac{2}{13}
\\\Large\text{1050}\normalsize\\
\lim_{x\to-8}{\frac{x^2-2x-80}{\sqrt{9x+136}-\sqrt{2x+80}}}=\\
\lim_{x\to-8}{\frac{(x^2-2x-80)(\sqrt{9x+136}-\sqrt{2x+80})}{9x+136-2x-80}}=\\
\lim_{x\to-8}{\frac{(x^2-2x-80)(\sqrt{9x+136}+\sqrt{2x+80})}{7x+56}}=\\
16\lim_{x\to-8}{\frac{x^2-2x-80}{7x+56}}=\\
16\lim_{x\to-8}{\frac{2x-2}{7}}=\frac{16(-18)}{7}=-\frac{288}{7}
\\\Large\text{1051}\normalsize\\
\lim_{x\to-7}{\frac{2-\sqrt[3]{x+15}}{x^2+9x+14}}=\\
\lim_{x\to-7}{\frac{2-\sqrt[3]{x+15}}{(x+7)(x+2)}}=\\
-\frac{1}{5}\lim_{x\to-7}{\frac{2-\sqrt[3]{x+15}}{x+7}}=\\
-\frac{1}{5}\lim_{x\to-7}{-\frac{1}{3(x+15)^{2/3}}}=\\
-\frac{1}{5}\lim_{x\to-7}{-\frac{1}{3\cdot4}}=\frac{1}{60}
